src/Std/Sat/AIG/CachedGates.lean
@@ -49,32 +49,18 @@ Create an xor gate in the input AIG. This uses the builtin cache to enable autom
 sharing.
 -/
 def mkXorCached (aig : AIG α) (input : BinaryInput aig) : Entrypoint α :=
-  -- x xor y = (invert (x && y)) && (invert ((invert x) && (invert y)))
-  let res := aig.mkAndGateCached input
-  let aig := res.aig
-  let aux1Ref := res.ref
-  let input := input.cast <| by apply LawfulOperator.le_size (f := mkAndGateCached)
-  let res := aig.mkAndGateCached (input.invert true true)
-  let aig := res.aig
-  let aux2Ref := res.ref
-  let aux1Ref := aux1Ref.cast <| by apply LawfulOperator.le_size (f := mkAndGateCached)
-  aig.mkAndGateCached ⟨aux1Ref.not, aux2Ref.not⟩
+  aig.mkXorGateCached input
 
 /--
 Create an equality gate in the input AIG. This uses the builtin cache to enable automated subterm
 sharing.
 -/
 def mkBEqCached (aig : AIG α) (input : BinaryInput aig) : Entrypoint α :=
-  -- a == b = (invert (a && (invert b))) && (invert ((invert a) && b))
-  let res := aig.mkAndGateCached <| input.invert false true
-  let aig := res.aig
-  let aux1Ref := res.ref
-  let input := input.cast <| by apply LawfulOperator.le_size (f := mkAndGateCached)
-  let res := aig.mkAndGateCached (input.invert true false)
-  let aig := res.aig
-  let aux2Ref := res.ref
-  let aux1Ref := aux1Ref.cast <| by apply LawfulOperator.le_size (f := mkAndGateCached)
-  aig.mkAndGateCached ⟨aux1Ref.not, aux2Ref.not⟩
+  -- a == b = !(a ^^ b)
+  let neq := aig.mkXorGateCached input
+  let aig := neq.aig
+  let ref := neq.ref
+  ⟨aig, ref.not⟩
 
 /--
 Create an implication gate in the input AIG. This uses the builtin cache to enable automated subterm
