src/Std/Sat/AIG/CachedLemmas.lean
@@ -124,9 +124,8 @@ theorem mkConstCached_eval_eq_mkConst_eval {aig : AIG α} :
   simp only [mkConstCached, denote_mkConst]
   unfold denote denote.go
   split
-  · simp
-  · next heq => simp [aig.hconst] at heq
-  · next heq => simp [aig.hconst] at heq
+  all_goals
+  · next heq => simp [aig.hconst] at heq <;> simp
 
 /--
 If we find a cached and gate declaration in the AIG, denoting it is equivalent to denoting `AIG.mkAndGate`.
@@ -257,6 +256,126 @@ theorem mkAndGateCached_eval_eq_mkAndGate_eval {aig : AIG α} {input : BinaryInp
   · rw [mkAndGateCached.go_eval_eq_mkAndGate_eval]
     simp only [denote_mkAndGate]
     rw [Bool.and_comm]
+
+/--
+If we find a cached xor gate declaration in the AIG, denoting it is equivalent to denoting `AIG.mkXorGate`.
+-/
+theorem denote_mkXorGate_cached {aig : AIG α} {input} {hit} :
+    aig.cache.get? (.xor (.mk input.lhs.gate input.lhs.invert) (.mk input.rhs.gate input.rhs.invert)) = some hit
+      →
+    ⟦⟨aig, hit.idx, false, hit.hbound⟩, assign⟧
+      =
+    ⟦aig.mkXorGate input, assign⟧ := by
+  intros
+  have := hit.hvalid
+  simp only [denote_mkXorGate]
+  conv =>
+    lhs
+    unfold denote denote.go
+  split <;> simp_all [denote]
+
+theorem mkXorGateCached.go_le_size (aig : AIG α) (input : BinaryInput aig) :
+    aig.decls.size ≤ (go aig input).aig.decls.size := by
+  dsimp only [go]
+  split
+  · simp
+  · split <;> try simp [mkConstCached_le_size]
+    split
+    · simp [mkConstCached_le_size]
+    · simp
+
+/--
+`AIG.mkXorGateCached` never shrinks the underlying AIG.
+-/
+theorem mkXorGateCached_le_size (aig : AIG α) (input : BinaryInput aig)
+    : aig.decls.size ≤ (aig.mkXorGateCached input).aig.decls.size := by
+  dsimp only [mkXorGateCached]
+  split
+  · apply mkXorGateCached.go_le_size
+  · apply mkXorGateCached.go_le_size
+
+theorem mkXorGateCached.go_decl_eq (aig : AIG α) (input : BinaryInput aig) :
+    ∀ (idx : Nat) (h1) (h2), (go aig input).aig.decls[idx]'h1 = aig.decls[idx]'h2 := by
+    generalize hres : go aig input = res
+    unfold go at hres
+    dsimp only at hres
+    split at hres
+    · rw [← hres]
+      intros
+      simp
+    · split at hres
+      · rw [← hres]
+        intros
+        simp
+      · rw [← hres]
+        intros
+        simp
+      · split at hres
+        · rw [← hres]
+          intros
+          rw [AIG.LawfulOperator.decl_eq (f := AIG.mkConstCached)]
+        · rw [← hres]
+          dsimp only
+          intro idx h1 h2
+          rw [Array.getElem_push]
+          simp [h2]
+
+/--
+The AIG produced by `AIG.mkXorGateCached` agrees with the input AIG on all indices that are valid for
+both.
+-/
+theorem mkXorGateCached_decl_eq (aig : AIG α) (input : BinaryInput aig) :
+    ∀ (idx : Nat) (h1) (h2), (aig.mkXorGateCached input).aig.decls[idx]'h1 = aig.decls[idx]'h2 := by
+    generalize hres : mkXorGateCached aig input = res
+    unfold mkXorGateCached at hres
+    dsimp only at hres
+    split at hres
+    all_goals
+      rw [← hres]
+      intros
+      rw [mkXorGateCached.go_decl_eq]
+
+instance : LawfulOperator α BinaryInput mkXorGateCached where
+  le_size := mkXorGateCached_le_size
+  decl_eq := by
+    intros
+    apply mkXorGateCached_decl_eq
+
+theorem mkXorGateCached.go_eval_eq_mkXorGate_eval {aig : AIG α} {input : BinaryInput aig} :
+    ⟦go aig input, assign⟧ = ⟦aig.mkXorGate input, assign⟧ := by
+  simp only [go]
+  split
+  · next heq1 =>
+    rw [denote_mkXorGate_cached heq1]
+  · split
+    · next invert _ =>
+      by_cases invert
+      all_goals
+      · simp_all [denote_getConstant]
+    · next invert _ hconst =>
+      have := hconst invert
+      by_cases invert
+      all_goals
+      · simp_all [denote_getConstant]
+    · rcases input with ⟨⟨lhs, linv, hlgate⟩, ⟨rhs, rinv, hrgate⟩⟩
+      split
+      · by_cases (linv = rinv)
+        · simp_all
+        · next hne => simp_all [Bool.eq_not_of_ne hne]
+      · simp [mkXorGate, denote]
+
+/--
+The central equality theorem between `mkAndGateCached` and `mkAndGate`.
+-/
+@[simp]
+theorem mkXorGateCached_eval_eq_mkXorGate_eval {aig : AIG α} {input : BinaryInput aig} :
+    ⟦aig.mkXorGateCached input, assign⟧ = ⟦aig.mkXorGate input, assign⟧ := by
+  simp only [mkXorGateCached]
+  split
+  · rw [mkXorGateCached.go_eval_eq_mkXorGate_eval]
+  · rw [mkXorGateCached.go_eval_eq_mkXorGate_eval]
+    simp only [denote_mkXorGate]
+    rw [Bool.xor_comm]
 
 end AIG
 
